Added a well-formedness condition for objects

src/Prototype/Transaction.v
@@ -40,10 +40,42 @@ Section System.
         Transaction rq rsr rs ->
         exists trsinv, TransactionInv rq trsinv rsr.
 
+    (* NOTE: this well-formedness for [PMsg] is a bit narrow.
+     * Should be extended for real systems.
+     *)
+    Inductive WfPMsg: PMsg MsgT StateT -> Prop :=
+    | WpRqRq:
+        forall pmsg,
+          msg_rqrs (midOf pmsg) = Rq ->
+          forall st,
+            Forall (fun msg_out =>
+                      msg_rqrs msg_out = Rq /\
+                      (* need this? *) msg_rs (midOf pmsg) = msg_rq msg_out /\
+                      msg_rq (midOf pmsg) <> msg_rs msg_out) (outsOf pmsg st) ->
+            WfPMsg pmsg
+    | WpRqRs:
+        forall pmsg,
+          msg_rqrs (midOf pmsg) = Rq ->
+          forall msg_out,
+            (forall st, outsOf pmsg st = msg_out :: nil) ->
+            msg_rqrs msg_out = Rs ->
+            msg_rq (midOf pmsg) = msg_rq msg_out ->
+            msg_rs (midOf pmsg) = msg_rs msg_out ->
+            WfPMsg pmsg
+    | WpRs:
+        forall pmsg,
+          msg_rqrs (midOf pmsg) = Rs ->
+          WfPMsg pmsg.
+
+    Definition WfObj (obj: Object MsgT StateT) :=
+      (forall pmsg, obj_pmsg_ints obj pmsg -> WfPMsg pmsg) /\
+      (forall pmsg, obj_pmsg_exts obj pmsg -> WfPMsg pmsg).
+
   End PerObject.
 
   Theorem locally_disjoint_linear:
     forall obs,
+      Forall (fun obj => WfObj obj) obs ->
       Forall (fun obj => LocallyDisjoint obj) obs ->
       Linear obs.
   Proof.
